Much speedup by changing everything

Reflection.v
@@ -88,8 +88,7 @@ Proof.
   now destruct n as [].
 Qed.
 
-
-
+Locate ret.
 
 (*** Working in models of PA ***)
 
@@ -113,77 +112,74 @@ Section Models.
   Definition representsF (d:D) trm rho := eval rho trm = d.
   Definition representableF (d:D) := exists trm rho, representsF d trm rho.
 
-Definition mergeAnd (rho:nat -> D) (P Q : naryProp 0) : {phi:form & representsP phi rho P} -> {phi:form & representsP phi rho Q} -> {phi:form & @representsP 0 phi rho (P /\ Q)}.
+Inductive FailureMonad (A:Type) : Type := ret : A -> FailureMonad A | fail : string -> FailureMonad A.
+Arguments ret {_} _.
+Arguments fail {_} _.
+Definition bind {A B : Type} (k:FailureMonad A) (f:A -> FailureMonad B) := match k return FailureMonad B with fail x => fail x | ret k => f k end.
+Notation "x <- c1 ;; c2" := (bind c1 (fun x => c2)).
+
+Definition mergeAnd (rho:nat -> D) (P Q : naryProp 0) (fP fQ : form) : representsP fP rho P -> representsP fQ rho Q -> @representsP 0 (fP∧fQ) rho (P /\ Q).
 Proof.
-intros [phiP HP] [phiQ HQ].
-pose (phiP∧phiQ). exists f. destruct HP as [pPl pPr]. destruct HQ as [pQl pQr]. unfold f. split.
+intros HP HQ.
+destruct HP as [pPl pPr]. destruct HQ as [pQl pQr]. split.
 * intros [pP pQ]. split. now apply pPl. now apply pQl.
 * intros [pP pQ]. split. now apply pPr. now apply pQr.
 Defined.
 
-Definition mergeFalse (rho:nat -> D) : {phi:form & @representsP 0 phi rho False}.
-Proof. exists fal. easy. Defined.
+Definition mergeFalse (rho:nat -> D) : @representsP 0 fal rho False.
+Proof. easy. Defined.
 
-Definition mergeOr (rho:nat -> D) (P Q : naryProp 0) : {phi:form & representsP phi rho P} -> {phi:form & representsP phi rho Q} -> {phi:form & @representsP 0 phi rho (P \/ Q)}.
+Definition mergeOr (rho:nat -> D) (P Q : naryProp 0) (fP fQ : form) : representsP fP rho P -> representsP fQ rho Q -> @representsP 0 (fP∨fQ) rho (P \/ Q).
 Proof.
-intros [phiP HP] [phiQ HQ].
-pose (phiP∨phiQ). exists f. destruct HP as [pPl pPr]. destruct HQ as [pQl pQr]. unfold f. split.
+intros HP HQ.
+destruct HP as [pPl pPr]. destruct HQ as [pQl pQr]. split.
 * intros [pP|pQ]. left; now apply pPl. right; now apply pQl.
 * intros [pP|pQ]. left; now apply pPr. right; now apply pQr.
 Defined.
 
-Definition mergeImpl (rho:nat -> D) (P Q : naryProp 0) : {phi:form & representsP phi rho P} -> {phi:form & representsP phi rho Q} -> {phi:form & @representsP 0 phi rho (P -> Q)}.
+Definition mergeImpl (rho:nat -> D) (P Q : naryProp 0) (fP fQ : form) : representsP fP rho P -> representsP fQ rho Q -> @representsP 0 (fP --> fQ) rho (P -> Q).
 Proof.
-intros [phiP HP] [phiQ HQ].
-pose (phiP-->phiQ). exists f. destruct HP as [pPl pPr]. destruct HQ as [pQl pQr]. unfold f. split.
+intros HP HQ.
+destruct HP as [pPl pPr]. destruct HQ as [pQl pQr]. split.
 * intros PQ pP. apply pQl, PQ, pPr, pP.
 * cbn. intros pPQ pP. apply pQr, pPQ, pPl, pP.
 Defined.
 
-Definition mergeExists (rho:nat -> D) (P:naryProp 1) : {phi:form & representsP phi rho P} -> {phi:form & @representsP 0 phi rho (exists q:D, P q)}.
+Definition mergeExists (rho:nat -> D) (P:naryProp 1) (fP:form) : representsP fP rho P -> @representsP 0 (∃ fP) rho (exists q:D, P q).
 Proof.
-intros [phi pR].
-pose (∃ phi). exists f. split.
+intros pR. split.
 * intros [q Pq]. exists q. destruct (pR q) as [pRl pRr]. now apply pRl.
 * intros [q Pq]. exists q. destruct (pR q) as [pRl pRr]. now apply pRr.
 Defined.
-(*
-Definition mergeForall (rho:nat -> D) (P:naryProp 1) : {phi:form & representsP phi rho P} -> {phi:form & @representsP 0 phi rho (forall q:D, P q)}.
+
+Definition mergeZero (rho:nat -> D) : representsF (iO) zero rho.
 Proof.
-intros [phi pR].
-pose (∀ phi). exists f. split.
-* intros H q. destruct (pR q) as [pRl pRr]. now apply pRl, H.
-* intros H q. destruct (pR q) as [pRl pRr]. now apply pRr, H.
-Defined.*)
-
-Definition mergeZero (rho:nat -> D) :{phi:term & representsF (iO) phi rho}.
-Proof.
-exists zero. easy.
+easy.
 Defined.
 
-Definition mergeSucc (rho:nat -> D) (d:D) : {phi:term & representsF d phi rho} -> {phi:term & representsF (iσ d) phi rho}.
-Proof. intros [t pt].
-pose (σ t). exists t0. unfold t0. unfold representsF. cbn. now rewrite pt.
+Definition mergeSucc (rho:nat -> D) (d:D) (phi:term) : representsF d phi rho -> representsF (iσ d) (σ phi) rho.
+Proof. intros pt.
+unfold representsF. cbn. now rewrite pt.
 Defined.
 
-Definition mergeAdd (rho:nat -> D) (d1 d2:D) : {phi:term & representsF d1 phi rho} -> {phi:term & representsF d2 phi rho} -> {phi:term & representsF (d1 i⊕ d2) phi rho}.
-Proof. intros [t1 pt1] [t2 pt2].
-pose (t1 ⊕ t2). exists t. unfold t. unfold representsF. cbn. now rewrite pt1, pt2.
+Definition mergeAdd (rho:nat -> D) (d1 d2:D) (t1 t2 : term) : representsF d1 t1 rho -> representsF d2 t2 rho -> representsF (d1 i⊕ d2) (t1⊕t2) rho.
+Proof. intros pt1 pt2.
+unfold representsF. cbn. now rewrite pt1, pt2.
 Defined.
 
-Definition mergeMul (rho:nat -> D) (d1 d2:D) : {phi:term & representsF d1 phi rho} -> {phi:term & representsF d2 phi rho} -> {phi:term & representsF (d1 i⊗ d2) phi rho}.
-Proof. intros [t1 pt1] [t2 pt2].
-pose (t1 ⊗ t2). exists t. unfold t. unfold representsF. cbn. now rewrite pt1, pt2.
+Definition mergeMul (rho:nat -> D) (d1 d2:D) (t1 t2 : term) : representsF d1 t1 rho -> representsF d2 t2 rho -> representsF (d1 i⊗ d2) (t1⊗t2) rho.
+Proof. intros pt1 pt2.
+unfold representsF. cbn. now rewrite pt1, pt2.
 Defined.
 
-Definition mergeEq (rho:nat -> D) (d1 d2 : D) : {phi:term & representsF d1 phi rho} -> {phi:term & representsF d2 phi rho} -> {phi:form & @representsP 0 phi rho (d1 i= d2)}.
-Proof. intros [t1 pt1] [t2 pt2].
-pose (t1 == t2). exists f. cbn. now rewrite pt1, pt2.
+Definition mergeEq (rho:nat -> D) (d1 d2 : D) (t1 t2 : term) : representsF d1 t1 rho -> representsF d2 t2 rho -> @representsP 0 (t1==t2) rho (d1 i= d2).
+Proof. intros pt1 pt2.
+cbn. now rewrite pt1, pt2.
 Defined.
 
-Definition mergeEqProp (rho:nat -> D) (d1 d2 : D) : {phi:term & representsF d1 phi rho} -> {phi:term & representsF d2 phi rho} -> {phi:form & @representsP 0 phi rho (d1 = d2)}.
-Proof. intros [t1 pt1] [t2 pt2].
-pose (t1 == t2). exists f. cbn. now rewrite pt1, pt2.
+Definition mergeEqProp (rho:nat -> D) (d1 d2 : D) (t1 t2 : term) : representsF d1 t1 rho -> representsF d2 t2 rho -> @representsP 0 (t1==t2) rho (d1 = d2).
+Proof. intros pt1 pt2.
+cbn. now rewrite pt1, pt2.
 Defined.
 
 Notation vectorCons x T n xr := 
@@ -206,10 +202,10 @@ Definition termPropRepStart :=
    tConst (MPfile (["Reflection"; "Arith"]), "PA_preds_signature") nil; tVar "D"; 
    tVar "I"]).
 
-Fixpoint recoverVector (f : Ast.term) {struct f}: TemplateMonad (list Ast.term) := let fail := tmPrint f;;tmFail "not a vector application" in match f with
+Fixpoint recoverVector (f : Ast.term) {struct f}: FailureMonad (list Ast.term) := let ffail := fail "not a vector application" in match f with
   vectorNil _ => ret nil
 | vectorCons x _ _ xr => xrl <- recoverVector xr;;ret (x::xrl)
-| _ => fail
+| _ => ffail
 end.
 
 Existing Instance config.default_checker_flags.
@@ -220,121 +216,114 @@ Fixpoint popListStart (l : list Ast.term) (ls : list Ast.term) : option (list As
 
 Definition FUEL := 100. 
 
-Definition termReifier := list Ast.term -> Ast.term -> (Ast.term -> TemplateMonad (prod term Ast.term)) -> TemplateMonad (prod term Ast.term).
-Definition reifyZero : termReifier := fun l env fTR => match l with nil => v <- tmQuote mergeZero;;ret (pair (zero) (tApp (v) ([env]))) | _ => tmFail "Zero constructor applied to != 0 terms" end.
+Definition termReifier := list Ast.term -> Ast.term -> (Ast.term -> FailureMonad (prod Ast.term Ast.term)) -> FailureMonad (prod Ast.term Ast.term).
+MetaCoq Quote Definition qMergeZero := mergeZero.
+MetaCoq Quote Definition qMergeZeroTerm := zero.
+Definition reifyZero : termReifier := fun l env fTR => match l with nil => ret ((qMergeZeroTerm, tApp (qMergeZero) ([env]))) | _ => fail "Zero constructor applied to != 0 terms" end.
+MetaCoq Quote Definition qMergeSucc := mergeSucc.
+MetaCoq Quote Definition qMergeSuccTerm := (fun k => σ k).
 Definition reifySucc : termReifier := fun l env fTR => match l with [x] => 
-                                           v <- tmQuote (mergeSucc);;
-                                           '(tx,xr) <- fTR x ;; ret (σ tx,tApp v ([env;x;xr])) | _ => tmFail "Succ constructor applied to != 1 terms" end.
+                                           k <- fTR x ;; let '(xt,xr) := k in ret (tApp qMergeSuccTerm ([xt]),tApp qMergeSucc ([env;x;xt;xr])) | _ => fail "Succ constructor applied to != 1 terms" end.
+MetaCoq Quote Definition qMergeAdd := mergeAdd.
+MetaCoq Quote Definition qMergeAddTerm := (fun k l => k⊕l).
 Definition reifyAdd : termReifier := fun l env fTR => match l with [x; y] =>  
-                                           v <- tmQuote (mergeAdd) ;;
-                                           '(tx,xr) <- fTR x ;; '(ty,yr) <- fTR y ;; ret (tx⊕ty,tApp v ([env;x;y;xr;yr])) | _ => tmFail "Add constructor applied to != 2 terms" end.
-Definition reifyMul : termReifier := fun l env fTR => match l with [x; y] =>  
-                                           v <- tmQuote (mergeMul) ;;
-                                           '(tx,xr) <- fTR x ;; '(ty,yr) <- fTR y ;; ret (tx⊗ty,tApp v ([env;x;y;xr;yr])) | _ => tmFail "Mul constructor applied to != 2 terms" end.
+                                           kx <- fTR x ;; ky <- fTR y ;; let '((xt,xp),(yt,yp)) := (kx,ky) in ret (tApp qMergeAddTerm ([xt;yt]), tApp qMergeAdd ([env;x;y;xt;yt;xp;yp])) | _ => fail "Add constructor applied to != 2 terms" end.
+MetaCoq Quote Definition qMergeMul := mergeMul.
+MetaCoq Quote Definition qMergeMulTerm := (fun k l => k⊗l).
+Definition reifyMul : termReifier := fun l env fTR => match l with [x; y] =>
+                                           kx <- fTR x ;; ky <- fTR y ;; let '((xt,xp),(yt,yp)) := (kx,ky) in ret (tApp qMergeMulTerm ([xt;yt]), tApp qMergeMul ([env;x;y;xt;yt;xp;yp])) | _ => fail "Mul constructor applied to != 2 terms" end.
 Definition reifyTerm (n:nat) : termReifier := match n with
-0 => reifyZero | 1 => reifySucc | 2 => reifyAdd | 3 => reifyMul | _ => fun _ _ _ => tmFail ("Unknown term constructor index " ++ string_of_nat n) end.
-Definition reifyRelHelper (rho:nat -> D) (d:D) (n:nat) (H:rho n = d) : {phi:term & representsF d phi rho}.
+0 => reifyZero | 1 => reifySucc | 2 => reifyAdd | 3 => reifyMul | _ => fun _ _ _ => fail ("Unknown term constructor index " ++ string_of_nat n) end.
+MetaCoq Quote Definition qMergeVarTerm := var.
+Definition reifyRelHelper (rho:nat -> D) (d:D) (n:nat) (H:rho n = d) : representsF d ($n) rho.
 Proof.
-exists ($n). exact H.
+exact H.
 Defined.
+MetaCoq Quote Definition qRelHelper := reifyRelHelper.
+MetaCoq Quote Definition qNatZero := 0.
+MetaCoq Quote Definition qNatSucc := S.
 
-
+Fixpoint quoteNumber (n:nat) : Ast.term:= match n with 0 => qNatZero | S n => tApp qNatSucc ([quoteNumber n]) end.
 
 Notation termRepDet i v := (([tConstruct {| inductive_mind := (MPfile (["Reflection"; "Arith"]), "PA_funcs"); inductive_ind := 0 |}
      i nil; v])).
 Notation formRepDet i v := (([tConstruct {| inductive_mind := (MPfile (["Reflection"; "Arith"]), "PA_preds"); inductive_ind := 0 |}
      i nil; v])).
-MetaCoq Quote Definition zeroEnv := (fun k:nat => iO).
 MetaCoq Quote Definition qeq_refl := (@eq_refl).
 
-Fixpoint findTermRepresentation (fuel:nat) (t:Ast.term) (termEnv:Ast.term) (env:Ast.term -> TemplateMonad nat) {struct fuel}: (TemplateMonad (prod term Ast.term)) := 
-  let fail := (v <- tmQuote reifyRelHelper;;envv <- env (t);;num <- tmQuote (envv);;ret ($envv,tApp v ([termEnv;t;num;tApp qeq_refl ([tVar "D";t])]))) in match fuel with 
-    0 => tmFail "Out of fuel" 
+Fixpoint findTermRepresentation (fuel:nat) (t:Ast.term) (termEnv:Ast.term) (env:Ast.term -> FailureMonad nat) {struct fuel}: (FailureMonad (prod Ast.term Ast.term)) := 
+  let ffail := (envv <- env (t);;let num := quoteNumber (envv) in ret (tApp qMergeVarTerm ([num]),tApp qRelHelper ([termEnv;t;num;tApp qeq_refl ([tVar "D";t])]))) in match fuel with 
+    0 => fail "Out of fuel" 
     | S fuel => match t with
         tApp termConstructorBase l => match popListStart l termPropRepStart with
           Some (termRepDet i v) => vr <- recoverVector v;;reifyTerm i vr termEnv (fun t => findTermRepresentation fuel t termEnv env)
-         | _ => fail end
-      | _ => fail
+         | _ => ffail end
+      | _ => ffail
     end 
   end.
 
 
+
 Definition proj1 {A:Type} {B:A -> Type} : {a:A & B a} -> A := fun z => match z with existT x _ => x end.
-Definition mergeForall2 (rho:nat -> D) (Q:naryProp 0) (H:{PP : naryProp 1 & (forall x:D, PP x) <-> Q}) : {phi:form & representsP phi rho (proj1 H)} -> {phi:form & @representsP 0 phi rho Q}.
+Definition mergeForall (rho:nat -> D) (Q:naryProp 0) (H:{PP : naryProp 1 & (forall x:D, PP x) <-> Q}) (phi:form) : representsP phi rho (proj1 H) -> @representsP 0 (∀ phi) rho Q.
 Proof.
-intros [phi pR]. destruct H as [PP [eql eqr]]. cbn in pR.
-pose (∀ phi). exists f. split.
+intros pR. destruct H as [PP [eql eqr]]. cbn in pR. split.
 * intros H q. destruct (pR q) as [pRl pRr]. now apply pRl, eqr, H.
 * intros H. apply eql. intros q. destruct (pR q) as [pRl pRr]. now apply pRr, H.
 Defined.
 
-
-(*
-Definition representForallP (Q:Prop) := a <- tmQuote (Q);; aa <- abstractForall a;;p <- tmUnquoteTyped ({P:naryProp 1 & (forall d:D, P d) <-> Q}) aa;; ret p.
-
-MetaCoq Run (let Q:=forall x:D, x i= iO in 
-    representForallP Q).
-
-Ltac representForall k:= match goal with [ k : ?Q |- _ ] =>
-  let fr := fresh "rep" in let kkk := fresh "sml" in let pr := fresh "denv" in let k y := (pose y as fr) in
-  (run_template_program (representForallP Q) k)
-  end.
-
-Lemma stuff : true.
-pose (forall x:nat, x > 0).
-(run_template_program (representForallP (forall x : D, x i= iO)) (let k y := (pose y) in k)).
-
-
-Definition lol := iO.
-MetaCoq Quote Definition lolEnv := (fun n:nat => lol).
-Definition phiRepr (rho:nat -> D) (t:D) := {phi:term & representsF t phi rho}.
-MetaCoq Run (let trm := lol i⊕ (iσ iO) in a <- tmQuote (trm);;
-v <- findTermRepresentation FUEL a lolEnv (fun _:Ast.term => ret 0);;k<-tmUnquoteTyped (phiRepr (fun n:nat => lol) trm) v;;tmDefinition "aa" k).
-*)
-
-Definition envTermReifier := list Ast.term -> nat -> Ast.term -> (Ast.term -> TemplateMonad nat) -> (Ast.term -> TemplateMonad (prod form Ast.term)) -> TemplateMonad (prod form Ast.term).
+Definition envTermReifier := list Ast.term -> nat -> Ast.term -> (Ast.term -> FailureMonad nat) -> (Ast.term -> FailureMonad (prod Ast.term Ast.term)) -> FailureMonad (prod Ast.term Ast.term).
+MetaCoq Quote Definition qMergeEq := mergeEq.
+MetaCoq Quote Definition qMergeFormEq := (fun a b => a == b).
 Definition refiyEq : envTermReifier := fun l fuel envTerm env fPR => match l with [x; y] =>  
-                                           v <- tmQuote mergeEq;;
-                                           '(tx,xr) <- findTermRepresentation fuel x envTerm env ;;
-                                           '(ty,yr) <- findTermRepresentation fuel y envTerm env ;; 
-                                           ret (tx==ty,tApp v ([envTerm;x;y;xr;yr])) | _ => tmFail "Eq constructor applied to != 2 terms" end.
-Definition reifyForm (n:nat) : envTermReifier := match n with 0 => refiyEq | _ => fun _ _ _ _ _ => tmFail ("Unknown form constructor index " ++ string_of_nat n) end.
+                                           (xr) <- findTermRepresentation fuel x envTerm env ;;
+                                           (yr) <- findTermRepresentation fuel y envTerm env ;; let '((xt,xp),(yt,yp)) := (xr,yr) in
+                                           ret (tApp qMergeFormEq ([xt;yt]), tApp qMergeEq ([envTerm;x;y;xt;yt;xp;yp])) | _ => fail "Eq constructor applied to != 2 terms" end.
+Definition reifyForm (n:nat) : envTermReifier := match n with 0 => refiyEq | _ => fun _ _ _ _ _ => fail ("Unknown form constructor index " ++ string_of_nat n) end.
 
 Notation baseLogicConn x l:= (tInd {| inductive_mind := (MPfile (["Logic"; "Init"; "Coq"]), x); inductive_ind := 0 |} l).
-Definition baseConnectiveReifier := list Ast.term -> nat -> Ast.term -> (Ast.term -> TemplateMonad nat) -> (Ast.term -> nat -> Ast.term -> (Ast.term -> TemplateMonad nat) -> TemplateMonad (prod form Ast.term))-> TemplateMonad (prod form Ast.term).
-Definition reifyAnd : baseConnectiveReifier := fun lst _ envTerm env fPR => match lst with [x; y] => v <- tmQuote mergeAnd;;
-                                           '(tx,xr) <- fPR x 0 envTerm env;;'(ty,yr) <- fPR y 0 envTerm env;; ret (tx∧ty,tApp v ([envTerm;x;y;xr;yr])) | _ => tmFail "And applied to != 2 terms" end.
-Definition reifyOr  : baseConnectiveReifier := fun lst _ envTerm env fPR => match lst with [x; y] => v <- tmQuote mergeOr;;
-                                           '(tx,xr) <- fPR x 0 envTerm env;;'(ty,yr) <- fPR y 0 envTerm env;; ret (tx∨ty,tApp v ([envTerm;x;y;xr;yr])) | _ => tmFail "Or applied to != 2 terms" end.
-Definition reifyExist:baseConnectiveReifier := fun lst _ envTerm env fPR => match lst with [_; P] => v <- tmQuote mergeExists;;
-                                           '(tP,rr) <- fPR P 1 envTerm env;; ret (∃ tP,tApp v ([envTerm;P;rr])) | _ => tmFail "Exist applied to wrong terms" end.
-Definition refiyCoqEq : baseConnectiveReifier := fun l fuel envTerm env fPR => match l with [tVar "D"; x; y] =>  
-                                           v <- tmQuote mergeEqProp;;
-                                           '(tx,xr) <- findTermRepresentation fuel x envTerm env ;;
-                                           '(ty,yr) <- findTermRepresentation fuel y envTerm env ;; 
-                                           ret (tx==ty,tApp v ([envTerm;x;y;xr;yr])) | _ => tmFail "Eq constructor applied to != 2 terms" end.
-Definition reifyBase (s:string) : baseConnectiveReifier := match s with "and" => reifyAnd | "or" => reifyOr | "ex" => reifyExist | "eq" => refiyCoqEq | _ => fun _ _ _ _ _ => tmFail ("Unknown connective "++s) end.
+Definition baseConnectiveReifier := list Ast.term -> nat -> Ast.term -> (Ast.term -> FailureMonad nat) -> (Ast.term -> nat -> Ast.term -> (Ast.term -> FailureMonad nat) -> FailureMonad (prod Ast.term Ast.term))-> FailureMonad (prod Ast.term Ast.term).
+MetaCoq Quote Definition qMergeAnd := mergeAnd.
+MetaCoq Quote Definition qMergeFormAnd := (fun a b => a∧b).
+Definition reifyAnd : baseConnectiveReifier := fun lst _ envTerm env fPR => match lst with [x; y] => 
+                                           xr <- fPR x 0 envTerm env;;yr <- fPR y 0 envTerm env;; let '((xt,xp),(yt,yp)) := (xr,yr) in
+                                           ret (tApp qMergeFormAnd ([xt;yt]), tApp qMergeAnd ([envTerm;x;y;xt;yt;xp;yp])) | _ => fail "And applied to != 2 terms" end.
+MetaCoq Quote Definition qMergeOr := mergeOr.
+MetaCoq Quote Definition qMergeFormOr := (fun a b => a∨b).
+Definition reifyOr  : baseConnectiveReifier := fun lst _ envTerm env fPR => match lst with [x; y] => 
+                                           xr <- fPR x 0 envTerm env;;yr <- fPR y 0 envTerm env;; let '((xt,xp),(yt,yp)) := (xr,yr) in
+                                           ret (tApp qMergeFormOr ([xt;yt]),tApp qMergeOr ([envTerm;x;y;xt;yt;xp;yp])) | _ => fail "Or applied to != 2 terms" end.
+MetaCoq Quote Definition qMergeExists := mergeExists.
+MetaCoq Quote Definition qMergeFormExists := (fun k => ∃k).
+Definition reifyExist:baseConnectiveReifier := fun lst _ envTerm env fPR => match lst with [_; P] => 
+                                           rr <- fPR P 1 envTerm env;; let '(rt,rp) := rr in 
+                                           ret (tApp qMergeFormExists ([rt]), tApp qMergeExists ([envTerm;P;rt;rp])) | _ => fail "Exist applied to wrong terms" end.
+MetaCoq Quote Definition qMergeEqProp := mergeEqProp.
+Definition refiyCoqEq : baseConnectiveReifier := fun l fuel envTerm env fPR => match l with [tVar "D"; x; y] => 
+                                           xr <- findTermRepresentation fuel x envTerm env ;;
+                                           yr<- findTermRepresentation fuel y envTerm env ;; let '((xt,xp),(yt,yp)) := (xr,yr) in
+                                           ret (tApp qMergeFormEq ([xt;yt]), tApp qMergeEqProp ([envTerm;x;y;xt;yt;xp;yp])) | _ => fail "Eq constructor applied to != 2 terms" end.
+Definition reifyBase (s:string) : baseConnectiveReifier := match s with "and" => reifyAnd | "or" => reifyOr | "ex" => reifyExist | "eq" => refiyCoqEq | _ => fun _ _ _ _ _ => fail ("Unknown connective "++s) end.
 
 
-Fixpoint raiseRelIndex (minn:nat) (t:Ast.term) : Ast.term := match t with
-  tRel n => if Compare_dec.le_gt_dec minn n then tRel (S n) else tRel n
+Fixpoint addRelIndex (minn:nat) (amnt:nat) (t:Ast.term) : Ast.term := match t with
+  tRel n => if Compare_dec.le_gt_dec minn n then tRel (amnt+n) else tRel n
 | tVar k => tVar k
-| tEvar n ls => tEvar n (map (raiseRelIndex minn) ls)
+| tEvar n ls => tEvar n (map (addRelIndex minn amnt) ls)
 | tSort u => tSort u
-| tCast t ck t2 => tCast (raiseRelIndex minn t) ck (raiseRelIndex minn t2)
-| tProd n t v => tProd n (raiseRelIndex minn t) (raiseRelIndex (S minn) v)
-| tLambda n t v => tLambda n (raiseRelIndex minn t) (raiseRelIndex (S minn) v)
-| tLetIn n t v e => tLetIn n (raiseRelIndex minn t) (raiseRelIndex minn v) (raiseRelIndex (S minn) e)
-| tApp f al => tApp f (map (raiseRelIndex minn) al)
+| tCast t ck t2 => tCast (addRelIndex minn amnt t) ck (addRelIndex minn amnt t2)
+| tProd n t v => tProd n (addRelIndex minn amnt t) (addRelIndex (S minn) amnt v)
+| tLambda n t v => tLambda n (addRelIndex minn amnt t) (addRelIndex (S minn) amnt v)
+| tLetIn n t v e => tLetIn n (addRelIndex minn amnt t) (addRelIndex minn amnt v) (addRelIndex (S minn) amnt e)
+| tApp f al => tApp (addRelIndex minn amnt f) (map (addRelIndex minn amnt) al)
 | tConst a b => tConst a b
 | tInd i t => tInd i t
 | tConstruct a b c => tConstruct a b c
-| tCase k i r m => tCase k (raiseRelIndex minn i) (raiseRelIndex minn r) (map (fun '(a,b) => (a,raiseRelIndex minn b)) m)
-| tProj p t => tProj p (raiseRelIndex minn t)
-| tFix mft n => tFix (map (map_def (raiseRelIndex minn) (raiseRelIndex (S minn))) mft) n
-| tCoFix mft n => tCoFix (map (map_def (raiseRelIndex minn) (raiseRelIndex (S minn))) mft) n
+| tCase k i r m => tCase k (addRelIndex minn amnt i) (addRelIndex minn amnt r) (map (fun '(a,b) => (a,addRelIndex minn amnt b)) m)
+| tProj p t => tProj p (addRelIndex minn amnt t)
+| tFix mft n => tFix (map (map_def (addRelIndex minn amnt) (addRelIndex (S minn) amnt)) mft) n
+| tCoFix mft n => tCoFix (map (map_def (addRelIndex minn amnt) (addRelIndex (S minn) amnt)) mft) n
 end.
-
 
 Notation qProp := (tSort (Universe.from_kernel_repr (Level.lProp, false) nil)).
 
@@ -342,34 +331,32 @@ MetaCoq Quote Definition qnaryProp1 := Eval compute in (naryProp 1).
 MetaCoq Quote Definition qexistT := @existT.
 MetaCoq Quote Definition qiff := @iff.
 MetaCoq Quote Definition qcong := @conj.
-(*MetaCoq Test Quote (@existT (naryProp 1) (fun P => (forall d:D, P d) <-> (forall d:D,False)) (fun _ => False) (conj (fun (k:(forall d:D,False))=>k) (fun (k:(forall d:D,False))=>k))).*)
 
-Definition abstractForall (t:Ast.term) : TemplateMonad (Ast.term) :=
+Definition abstractForall (t:Ast.term) : FailureMonad (Ast.term) :=
 match t with tProd x t v =>
     let prop := tLambda x t v in
-    let raisedV := raiseRelIndex 0 (tProd x t v) in
-    ret (tApp (qexistT) ([qnaryProp1; tLambda (nNamed "P") qnaryProp1 (tApp qiff 
-                ([tProd x t (tApp (tRel 1) ([tRel 0])); raisedV]));
-                 tLambda x t v; tApp qcong ([
-tProd (nNamed "x") (tProd x t v) raisedV;
-tProd (nNamed "x") (tProd x t v) raisedV;
-tLambda (nNamed "k") (tProd x t v) (tRel 0);
-tLambda (nNamed "k") (tProd x t v) (tRel 0)
-])]))
-| _ => tmPrint t;;tmFail "called abstractForall on something not a product" end.
+    ret (tLetIn (nNamed "Q") (tProd x t v) qProp (tApp (qexistT) ([qnaryProp1; tLambda (nNamed "P") qnaryProp1 (tApp qiff 
+                ([tProd x (addRelIndex 0 2 t) (tApp (tRel 1) ([tRel 0])); tRel 1]));
+                 addRelIndex 0 1 (prop); tApp qcong ([
+tProd (nNamed "x") (tRel 0) (tRel 1);
+tProd (nNamed "x") (tRel 0) (tRel 1);
+tLambda (nNamed "k") (tRel 0) (tRel 0);
+tLambda (nNamed "k") (tRel 0) (tRel 0)
+])])))
+| _ => fail "called abstractForall on something not a product" end.
 
 
 Definition pred (n:nat) := match n with 0 => 0 | S n => n end.
-Fixpoint flatten_monad {A:Type} (l:list (TemplateMonad A)) : TemplateMonad (list A) := match l with nil => ret nil | x::xr => xm <- x;; xrm <- flatten_monad xr;; ret (xm::xrm) end.
-Definition map_monad {A B:Type} (f:A -> TemplateMonad B) (l:list A) : TemplateMonad (list B) := flatten_monad (map f l).
-Definition map_def_monad {A B : Type} (tyf bodyf : A -> TemplateMonad B) (d:def A) : TemplateMonad (def B) := dtr <- tyf (dbody d);;dbr <- bodyf (dbody d);; ret {|
+Fixpoint flatten_monad {A:Type} (l:list (FailureMonad A)) : FailureMonad (list A) := match l with nil => ret nil | x::xr => xm <- x;; xrm <- flatten_monad xr;; ret (xm::xrm) end.
+Definition map_monad {A B:Type} (f:A -> FailureMonad B) (l:list A) : FailureMonad (list B) := flatten_monad (map f l).
+Definition map_def_monad {A B : Type} (tyf bodyf : A -> FailureMonad B) (d:def A) : FailureMonad (def B) := dtr <- tyf (dbody d);;dbr <- bodyf (dbody d);; ret {|
 dname := dname d;
 dtype := dtr;
 dbody := dbr;
 rarg := rarg d |}.
-Check (Compare_dec.le_gt_dec).
-Fixpoint lowerRelIndex (minn:nat) (tv:TemplateMonad Ast.term) (t:Ast.term) {struct t}: TemplateMonad Ast.term := match t with
-  tRel n => if Compare_dec.le_gt_dec minn n then if Compare_dec.le_gt_dec minn (S n) then tmPrint "pred";;tmPrint (tRel (pred n));;ret (tRel (pred n)) else tmPrint (minn,n);;tv else tmPrint "inside";;ret (tRel n)
+
+Fixpoint lowerRelIndex (minn:nat) (tv:FailureMonad Ast.term) (t:Ast.term) {struct t}: FailureMonad Ast.term := match t with
+  tRel n => if Compare_dec.le_gt_dec minn n then if Compare_dec.le_gt_dec minn (S n) then ret (tRel (pred n)) else tv else ret (tRel n)
 | tVar k => ret (tVar k)
 | tEvar n ls => m <- map_monad (lowerRelIndex minn tv) ls;;ret (tEvar n m)
 | tSort u => ret (tSort u)
@@ -377,7 +364,7 @@ Fixpoint lowerRelIndex (minn:nat) (tv:TemplateMonad Ast.term) (t:Ast.term) {stru
 | tProd n t v => mt<-(lowerRelIndex minn tv t);;mv<-(lowerRelIndex (S minn) tv v);;ret (tProd n mt mv)
 | tLambda n t v => mt<-(lowerRelIndex minn tv t);;mv<-(lowerRelIndex (S minn) tv v);;ret (tLambda n mt mv)
 | tLetIn n t v e => mt<-(lowerRelIndex minn tv t);;mv<-(lowerRelIndex minn tv v);;me<-(lowerRelIndex (S minn) tv e);;ret (tLetIn n mt mv me)
-| tApp f al => mal<-(map_monad (lowerRelIndex minn tv) al);;ret (tApp f mal)
+| tApp f al => mal<-(map_monad (lowerRelIndex minn tv) al);;ff <- lowerRelIndex minn tv f;;ret (tApp ff mal)
 | tConst a b => ret (tConst a b)
 | tInd i t => ret (tInd i t)
 | tConstruct a b c => ret (tConstruct a b c)
@@ -387,85 +374,126 @@ Fixpoint lowerRelIndex (minn:nat) (tv:TemplateMonad Ast.term) (t:Ast.term) {stru
 | tCoFix mft n => mmft<-(map_monad (map_def_monad (lowerRelIndex minn tv) (lowerRelIndex (S minn) tv)) mft);;ret (tCoFix mmft n)
 end.
 
-Definition appendZero (env:Ast.term -> TemplateMonad nat) (zv:TemplateMonad nat) : (Ast.term -> TemplateMonad nat) := 
-      fun (t:Ast.term) => match t with tRel n => (match n with 0 => zv | S n => env (tRel n) end) | _ => tmFail "stuff" end. (*k <- lowerRelIndex 0 (tmFail "Error 1337") t;; (env k) end.*)
-Definition appendAndLift (env:Ast.term -> TemplateMonad nat) (zv:TemplateMonad nat) : (Ast.term -> TemplateMonad nat) := 
-      fun t => match t with tRel n => (match n with 0 => zv | S n => k <- env (tRel n);;ret (S k) end) | _ => tmFail "stuff2" end. (*k <- lowerRelIndex 0 (tmFail "Error 1337") t;; v <- env k;;ret (S v) end.*)
-MetaCoq Quote Definition qraiseEnvTerm := (fun (d:D) (rho:nat -> D) => d .: rho).
-Definition raiseEnvTerm (d:Ast.term) (env:Ast.term) : Ast.term := tApp (qraiseEnvTerm) ([d;raiseRelIndex 0 env]).
-
-Definition mergeFreeVarIntro (rho:nat -> D) (n:nat) (P:naryProp (S n)) (H:forall d:D, {phi:form & representsP phi (d.:rho) (P d)}) (H2:forall d:D, proj1 (H iO) = proj1 (H d)) : {phi:form & representsP phi rho P}.
-Proof.
-pose (proj1 (H (iO))). exists f. intros k. destruct (H k) as [trm prf] eqn:Heq. specialize (H2 k). rewrite Heq in H2. cbn in H2. unfold f. rewrite H2. exact prf.
-Defined.
-MetaCoq Quote Definition qform := form.
+Definition appendZero (env:Ast.term -> FailureMonad nat) (zv:FailureMonad nat) : (Ast.term -> FailureMonad nat) := 
+      fun (t:Ast.term) => match t with tRel n => (match n with 0 => zv | S n => env (tRel n) end) | _ => k <- lowerRelIndex 0 (fail "tRel 0 used when lowering") t;; (env k) end.
+Definition appendAndLift (env:Ast.term -> FailureMonad nat) (zv:FailureMonad nat) : (Ast.term -> FailureMonad nat) := 
+      fun t => match t with tRel n => (match n with 0 => zv | S n => k <- env (tRel n);;ret (S k) end) | _ => k <- lowerRelIndex 0 (fail "tRel 0 used when lowering") t;; v <- env k;;ret (S v) end.
+Definition raiseEnvTermBase := (fun (d:D) (rho:nat -> D) => d .: rho).
+MetaCoq Test Quote (fun (d:D) (rho:nat -> D) => d .: rho).
+Definition qraiseEnvTerm := (tApp (tConst (MPfile (["FOL"; "Arith"]), "scons") nil) ([tVar "D"])).
+Definition raiseEnvTerm (d:Ast.term) (env:Ast.term) : Ast.term := tApp (qraiseEnvTerm) ([d;env]).
 (*
-
-Definition mergeForall2 (rho:nat -> D) (Q:naryProp 0) (H:{PP : naryProp 1 & (forall x:D, PP x) <-> Q}) : {phi:form & representsP phi rho (proj1 H)} -> {phi:form & @representsP 0 phi rho Q}.
+Axiom falsity : False.
+Definition mergeFreeVarIntro (rho:nat -> D) (n:nat) (P:naryProp (S n)) 
+                             (H:forall d:D, {phi:form & representsP phi (d.:rho) (P d)}) 
+                             (*(H2:forall d:D, proj1 (H iO) = proj1 (H d))*) : {phi:form & representsP phi rho P}.
 Proof.
-intros [phi pR]. destruct H as [PP [eql eqr]]. cbn in pR.
-pose (∀ phi). exists f. split.
-* intros H q. destruct (pR q) as [pRl pRr]. now apply pRl, eqr, H.
-* intros H. apply eql. intros q. destruct (pR q) as [pRl pRr]. now apply pRr, H.
+pose (proj1 (H (iO))). exists f. exfalso. exact falsity.
+(*intros k. destruct (H k) as [trm prf] eqn:Heq. specialize (H2 k). rewrite Heq in H2. cbn in H2. unfold f. rewrite H2. exact prf.*)
 Defined.
+Definition freeVarH2Proof (rho:nat -> D) (n:nat) (P:naryProp (S n)) (H:forall d:D, {phi:form & representsP phi (d.:rho) (P d)}) : forall d:D, proj1 (H d) = proj1 (H d).
+Proof. intros d. exact eq_refl. Defined.
+MetaCoq Quote Definition qVarIntro := mergeFreeVarIntro.
+MetaCoq Quote Definition qH2Proof := freeVarH2Proof.
 *)
+MetaCoq Quote Definition qMergeFalse := mergeFalse.
+MetaCoq Quote Definition qMergeForall := mergeForall.
+MetaCoq Quote Definition qMergeImpl := mergeImpl.
+MetaCoq Quote Definition qMergeFormFalse := fal.
+MetaCoq Quote Definition qMergeFormForall := (fun k => ∀ k).
+MetaCoq Quote Definition qMergeFormImpl := (fun p q => p --> q).
+MetaCoq Quote Definition qform := form.
+MetaCoq Quote Definition qenvType := (nat -> D).
+MetaCoq Quote Definition qProj1 := @proj1.
+MetaCoq Quote Definition qRepresentsP := @representsP.
+MetaCoq Quote Definition qNaryProp := @naryProp.
+MetaCoq Quote Definition qnat := nat.
+Definition fvType := (fun (rho:nat -> D) (n:nat) (P:naryProp (S n)) =>  forall d:D, {phi:form & representsP phi (d.:rho) (P d)}).
+MetaCoq Quote Definition qrepresentsT := fvType.
 
-Fixpoint findPropRepresentation (fuel:nat) (t:Ast.term) (frees:nat) (envTerm:Ast.term) (env:Ast.term -> TemplateMonad nat) {struct fuel}: (TemplateMonad (prod form Ast.term)) := tmPrint t;;
-let fail :=tmPrint (frees,t);;tmFail ("Cannot represent form") in match fuel with 0 => tmFail "Out of fuel" | S fuel => 
+Fixpoint findPropRepresentation (fuel:nat) (t:Ast.term) (frees:nat) (envTerm:Ast.term) (env:Ast.term -> FailureMonad nat) {struct fuel}: (FailureMonad (prod Ast.term Ast.term)) := 
+let ffail :=fail ("Cannot represent form") in match fuel with 0 => fail "Out of fuel" | S fuel => 
   match (frees,t) with
-  (0,(baseLogicConn "False" nil)) => v <- tmQuote mergeFalse;;ret (fal,tApp v ([envTerm]))
+  (0,(baseLogicConn "False" nil)) => ret (qMergeFormFalse, tApp qMergeFalse ([envTerm]))
 | (0,(tApp (baseLogicConn name nil) lst)) => reifyBase name lst fuel envTerm env (findPropRepresentation fuel)
 | (0,(tApp propConstructorBase lst)) => match popListStart lst termPropRepStart with
         Some (formRepDet i v) => vr <- recoverVector v;;reifyForm i vr fuel envTerm env (fun t => findPropRepresentation fuel t frees envTerm env)
-      | _ => fail end
-| (0,tProd x (tVar "D") Q) =>
-      k <- abstractForall (tProd x (tVar "D") Q);;
-      '(frm,tQ) <- findPropRepresentation fuel (tLambda x (tVar "D") Q) 1 envTerm env;;
-      v <- tmQuote mergeForall2;;
-      ret (∀ frm, tApp v ([envTerm;tProd x (tVar "D") Q;k;tQ]))
-| (0,tProd _ P Q) =>
-      v <- tmQuote mergeImpl;;
-      '(tP,rP) <- findPropRepresentation fuel P 0 envTerm env;;
-      Ql <- lowerRelIndex 0 (tmFail "Used var of implication precondition") Q;;
-      '(tQ,rQ) <- findPropRepresentation fuel Ql 0 envTerm env;;
-      ret (tP --> tQ,tApp v ([envTerm;P;Ql;rP;rQ]))
-| (S n,tLambda x (tVar "D") P) => 
-      let envTermSub := raiseEnvTerm (tRel 0) envTerm in
+      | _ => ffail end
+| (0,tProd x P Q) => if Checker.eq_term init_graph P (tVar "D") then
+                          k <- abstractForall (tProd x (tVar "D") Q);;
+                          rQ <- findPropRepresentation fuel (tLambda x (tVar "D") Q) 1 envTerm env;; let '(tQ,pQ) := rQ in
+                          ret (tApp qMergeFormForall ([tQ]), tApp qMergeForall ([envTerm;tProd x (tVar "D") Q;k;tQ;pQ]))
+                     else
+                          rP <- findPropRepresentation fuel P 0 envTerm env;;
+                          Ql <- lowerRelIndex 0 (fail "Used var of implication precondition") Q;;
+                          rQ <- findPropRepresentation fuel Ql 0 envTerm env;; let '((tP,pP),(tQ,pQ)) := (rP,rQ) in
+                          ret (tApp qMergeFormImpl ([tP;tQ]), tApp qMergeImpl ([envTerm;P;Ql;tP;tQ;pP;pQ]))
+| (S n,tLambda x T P) => if Checker.eq_term init_graph T (tVar "D") then
+      let envTermSub := raiseEnvTerm (tRel 0) (addRelIndex 0 1 envTerm) in
       let envSub := appendAndLift env (ret 0) in
-      '(frm,k) <- findPropRepresentation fuel P n envTermSub envSub;;
-      v <- tmQuote mergeFreeVarIntro;;
-      num <- tmQuote n;;
-      vfrmq <- tmQuote frm;;
-      ret (frm,tApp v ([envTerm;num;tLambda x (tVar "D") P;tLambda x (tVar "D") k;tLambda x (tVar "D") (tApp qeq_refl ([qform;vfrmq]))]))
-| _ => fail end end.
+      let num := quoteNumber n in
+      k <- findPropRepresentation fuel P n envTermSub envSub;; let '(tk,pk) := k in
+      ret (tk,(tLambda x (tVar "D") pk))
+     else ffail
+| _ => ffail end end.
 
-Check print_term.
-MetaCoq Quote Recursively Definition k := mergeFreeVarIntro.
-Check (fst k).
-Definition genv := empty_ext (fst k).
-
-Ltac representEnv env := match goal with [ |- representableP ?n ?G ] =>
-  let rep := fresh "rep" in let prf := fresh "prf" in let hyp := fresh "H" in let k y := (idtac y;destruct y as [rep prf]) in
-  (run_template_program (g <- (tmQuote G);;qe <- tmQuote env;;'(aaa,rp)<-findPropRepresentation FUEL g n qe (fun v => tmFail "unbound");;tmPrint (aaa,rp);;(*print_term genv nil false rp*)tmUnquoteTyped ({phi:form & @representsP n phi env G}) rp) k)
+Definition f2t {T:Type} (a:FailureMonad T) : TemplateMonad T := match a with ret k => monad_utils.ret k | fail s => tmFail s end.
+Check existT.
+Ltac representEnv env env2:= match goal with [ |- representableP ?n ?G ] =>
+  let rep := fresh "rep" in let prf := fresh "prf" in let hyp := fresh "hyp" in let k y := (destruct y as [rep prf]) in
+  (run_template_program (monad_utils.bind (tmQuote G) (fun g => 
+                         monad_utils.bind (tmQuote env) (fun qe => 
+                         monad_utils.bind (f2t (findPropRepresentation FUEL g n qe env2)) (fun '(tPq,pPq) => 
+                         monad_utils.bind (tmUnquoteTyped (form) tPq) (fun tP:form => 
+                         monad_utils.bind (tmUnquoteTyped (@representsP n tP env G) pPq) (fun tQ : @representsP n tP env G =>
+                         monad_utils.ret (@existT form (fun mm => @representsP n mm env G) tP tQ))))))) k)
   ;exists rep;exists env;exact prf
 end.
-Ltac represent := representEnv (fun k:nat => iO).
+Ltac represent := representEnv (fun k:nat => iO) (fun (v:Ast.term) => @fail nat "unbound").
 
 Goal (representableP 0 (iO i= iO)).
-represent.
+Time represent.
 Qed.
 
 Goal (representableP 0 (forall d:D, d i= iO)).
-represent.
+Time represent.
+Show Proof.
 Qed.
 
-Goal (representableP 1 (fun a => False -> a i= a)).
-represent.
+Goal (representableP 2 (fun a b  => a i= b)).
+Time represent. 
+Show Proof.
 Qed.
+
 
 Goal (representableP 2 (fun (d e :D) => forall g, exists j, g i= d i⊕ j /\ False -> False \/ (e i⊗ e i= iσ j /\ False))).
-represent.
+Time represent.
+Show Proof.
+Qed.
+Goal (representableP 0 (forall a b, a i= b)).
+Time represent. 
+Time Qed.
+Goal (representableP 0 (forall a b c, a i= b i⊕ c)).
+Time represent.
+Time Qed.
+Goal (representableP 0 (forall a b c d ,a i= b i⊕ c i⊕ d)).
+Time represent. 
+Time Qed.
+Goal (representableP 0 (forall a b c d e , a i= b i⊕ c i⊕ d i⊕ e)).
+Time represent. 
+Time Qed.
+Goal (representableP 0 (forall a b c d e f , a i= b i⊕ c i⊕ d i⊕ e i⊕ f)).
+Time represent. 
+Time Qed.
+Lemma test32 : (representableP 0 (forall a b c d e f g , a i= b i⊕ c i⊕ d i⊕ e i⊕ f i⊕ g)).
+Time represent. 
+Time Qed.
+Set Printing Depth 500.
+Print test32.
 
+Goal forall n m:D, (representableP 0 (n i= m)).
+intros n m. representEnv (fun k:nat => match k with 0 => n | _ => m end) (fun l:Ast.term => match l with (tVar "n") => ret 0 | (tVar "m") => ret 1 | _ => fail "unbound" end).
+Qed.
 
 Goal (forall n:nat, representableF (iμ n)).
 intros n. induction n as [|n [phi [rho IH]]].
@@ -550,13 +578,10 @@ Qed.
   Qed.
 
   Lemma add_rec_right :
-    forall d n, n i⊕ (iσ d) i= iσ (n i⊕ d).
+    forall d n, n i⊕ (iσ d) = iσ (n i⊕ d).
   Proof.
-    apply PAinduction.
-    - represent. pose (phi := ∀ $1 ⊕ σ $2 == σ ($1 ⊕ $2) ).
-      exists phi. exists (fun _ => n). intros d. cbn. split.
-      + intros H d0. rewrite equality. cbn. easy.
-      + intros H. specialize (H n). rewrite equality in H. cbn in H. auto.
+    intros n. apply PAinduction.
+    - representEnv (fun k:nat => n) (fun k:Ast.term => ret 0).
     - rewrite !add_zero; try reflexivity. all: firstorder.
     - intros d IH. rewrite !add_rec. now rewrite IH. all: firstorder.
   Qed.
